\chapter{Hund's Coupling Cases}
\label{c:hunds_coupling_cases}

\section{Hund's Case (a)}
\label{s:hunds_case_a}

\subsection{Good Quantum Numbers}

\begin{equation*}
    \Lambda, S, \Sigma, J, \Omega
\end{equation*}

\subsection{Selection Rules}

General rules
\begin{align*}
    g        &\nleftrightarrow g, \quad g \leftrightarrow u, \quad u \nleftrightarrow u \\
    \adif{J} &= 0, \pm 1 \text{ with the restriction } J = 0 \nrightarrow J = 0
\end{align*}

Rules common to both (a) and (b)
\begin{align*}
    \adif{\Lambda} &= 0, \pm 1 \\
    \adif{S}       &= 0
\end{align*}

Rules for case (a) only
\begin{align*}
    \adif{\Sigma} &= 0        \\
    \adif{\Omega} &= 0, \pm 1 \\
    \adif{J}      &= 0 \text{ is forbidden for } \Omega = 0 \rightarrow \Omega = 0
\end{align*}

\subsection{Term Values}

\begin{equation*}
    F_v(J) = B_v[J(J + 1) - \Omega^2]
\end{equation*}

\section{Hund's Case (b)}
\label{s:hunds_case_b}

\subsection{Good Quantum Numbers}

\begin{equation*}
    \Lambda, N, S, J
\end{equation*}

\subsection{Selection Rules}

General rules
\begin{align*}
    g        &\nleftrightarrow g, \quad g \leftrightarrow u, \quad u \nleftrightarrow u \\
    \adif{J} &= 0, \pm 1 \text{ with the restriction } J = 0 \nrightarrow J = 0
\end{align*}

Rules common to both (a) and (b)
\begin{align*}
    \adif{\Lambda} &= 0, \pm 1 \\
    \adif{S}       &= 0
\end{align*}

Rules for case (b) only
\begin{align*}
    \adif{N} &= 0, \pm 1 \\
    \adif{N} &= 0 \text{ is forbidden for } \Sigma\dash\Sigma \text{ transitions}
\end{align*}

\subsection{Term Values}

$\state{2}{\Sigma}$ states
\begin{align*}
    F_1(N) &= B_vN(N + 1) + \tfrac{1}{2}\gamma N \\
    F_2(N) &= B_vN(N + 1) - \tfrac{1}{2}\gamma(N + 1)
\end{align*}

$\state{3}{\Sigma}$ states
\begin{align*}
    F_1(N) &= B_vN(N + 1) + (2N + 3)B_v - \lambda - \sqrt{(2N + 3)^2B_v^2 + \lambda^2 - 2\lambda B_v} + \gamma(N + 1) \\
    F_2(N) &= B_vN(N + 1)                                                                                             \\
    F_3(N) &= B_vN(N + 1) - (2N - 1)B_v - \lambda + \sqrt{(2N - 1)^2B_v^2 + \lambda^2 - 2\lambda B_v} - \gamma N
\end{align*}
