\chapter{Uncoupling}
\label{c:uncoupling}

\section{\texorpdfstring{$\Lambda$}{Î›} Doubling}
\label{s:lambda_doubling}

\section{Spin Uncoupling}
\label{s:spin_uncoupling}

\subsection{Doublet States}

\begin{align*}
    F_1(J) &= B_v\bk*{\pr*{J + \tfrac{1}{2}}^2 - \Lambda^2 - \tfrac{1}{2}\sqrt{4\pr*{J + \tfrac{1}{2}}^2 + Y(Y - 4)\Lambda^2}} - D_vJ^4 \\
    F_2(J) &= B_v\bk*{\pr*{J + \tfrac{1}{2}}^2 + \Lambda^2 - \tfrac{1}{2}\sqrt{4\pr*{J + \tfrac{1}{2}}^2 + Y(Y - 4)\Lambda^2}} - D_v(J + 1)^4
\end{align*}

\subsection{Triplet States}

\begin{align*}
    F_1(J) &= B_v\bk*{J(J + 1) - \sqrt{Z_1} - 2Z_2} - D_v\pr*{J - \tfrac{1}{2}}^4 \\
    F_2(J) &= B_v[J(J + 1) + 4Z_2] - D_v\pr*{J + \tfrac{1}{2}}^4 \\
    F_3(J) &= B_v\bk*{J(J + 1) + \sqrt{Z_1} - 2Z_2} - D_v\pr*{J + \tfrac{3}{2}}^4
\end{align*}
where
\begin{align*}
    Z_1 &= \Lambda^2Y(Y - 4) + \tfrac{4}{3} + 4J(J + 1) \\
    Z_2 &= \frac{1}{3Z_1}\bk*{\Lambda^3Y(Y - 1) - \tfrac{4}{9} - 2J(J + 1)}
\end{align*}
